Superposition_Calculus/Abstract_Substitution/Variable_Substitution.thy
@@ -3,10 +3,10 @@ theory Variable_Substitution
 begin
 
 (* TODO: Better name?: functional substitution *)
-locale variable_substitution = basic_substitution _ _ subst "\<lambda>a.  vars a = {}"
-  for subst :: "'value \<Rightarrow> ('x \<Rightarrow> 'subvalue) \<Rightarrow> 'value" (infixl "\<cdot>" 70) and
+locale variable_substitution = basic_substitution _ _ subst "\<lambda>a. vars a = {}"
+  for subst :: "'value \<Rightarrow> ('variable \<Rightarrow> 'subvalue) \<Rightarrow> 'value" (infixl "\<cdot>" 70) and
     (* TODO: set \<rightarrow> fset *)
-      vars :: "'value \<Rightarrow> 'x set" +
+      vars :: "'value \<Rightarrow> 'variable set" +
   assumes
     subst_eq: "\<And>a \<sigma> \<tau>. (\<And>x. x \<in> vars a \<Longrightarrow> \<sigma> x = \<tau> x) \<Longrightarrow> a \<cdot> \<sigma> = a \<cdot> \<tau>" and
     finite_vars [simp]: "\<And>a. finite (vars a)"
@@ -17,7 +17,8 @@ abbreviation is_ground where "is_ground a \<equiv> vars a = {}"
 lemma subst_reduntant_upd [simp]:
   assumes "var \<notin> vars a"
   shows "a \<cdot> \<sigma>(var := update) = a \<cdot> \<sigma>"
-  using assms subst_eq by fastforce
+  using assms subst_eq 
+  by fastforce
 
 lemma subst_reduntant_if [simp]: 
   assumes "vars a \<subseteq> vars'"
@@ -41,7 +42,8 @@ locale variable_substitution_lifting = base: variable_substitution +
      comp_subst = comp_subst and 
      vars = lifted_vars 
   for lifted_subst lifted_vars  +
-  assumes lifted_vars_vars:  "(\<forall>x. lifted_vars (lifted_subst x \<gamma>) = {}) \<longleftrightarrow> (\<forall>x. vars (x \<cdot> \<gamma>) = {})"
+  assumes 
+    lifted_vars_vars: "(\<forall>x. lifted_vars (lifted_subst x \<gamma>) = {}) \<longleftrightarrow> (\<forall>x. vars (x \<cdot> \<gamma>) = {})"
 begin
 
 lemma is_ground_subst_iff [simp]: "is_ground_subst \<gamma> \<longleftrightarrow> base.is_ground_subst \<gamma>"
